src/HOL/MicroJava/BV/BVSpec.thy
@@ -17,42 +17,42 @@ text {*
 
 constdefs
   wt_instr :: "[instr,jvm_prog,ty,method_type,nat,p_count,
-                exception_table,p_count] => bool"
+                exception_table,p_count] \<Rightarrow> bool"
   "wt_instr i G rT phi mxs max_pc et pc == 
   app i G mxs rT pc et (phi!pc) \<and>
   (\<forall>(pc',s') \<in> set (eff i G pc et (phi!pc)). pc' < max_pc \<and> G \<turnstile> s' <=' phi!pc')"
 
-  wt_start :: "[jvm_prog,cname,ty list,nat,method_type] => bool"
+  wt_start :: "[jvm_prog,cname,ty list,nat,method_type] \<Rightarrow> bool"
   "wt_start G C pTs mxl phi == 
   G \<turnstile> Some ([],(OK (Class C))#((map OK pTs))@(replicate mxl Err)) <=' phi!0"
 
   wt_method :: "[jvm_prog,cname,ty list,ty,nat,nat,instr list,
-                 exception_table,method_type] => bool"
+                 exception_table,method_type] \<Rightarrow> bool"
   "wt_method G C pTs rT mxs mxl ins et phi ==
   let max_pc = length ins in
   0 < max_pc \<and> wt_start G C pTs mxl phi \<and> 
-  (\<forall>pc. pc<max_pc --> wt_instr (ins ! pc) G rT phi mxs max_pc et pc)"
+  (\<forall>pc. pc<max_pc \<longrightarrow> wt_instr (ins ! pc) G rT phi mxs max_pc et pc)"
 
-  wt_jvm_prog :: "[jvm_prog,prog_type] => bool"
+  wt_jvm_prog :: "[jvm_prog,prog_type] \<Rightarrow> bool"
   "wt_jvm_prog G phi ==
   wf_prog (\<lambda>G C (sig,rT,(maxs,maxl,b,et)).
            wt_method G C (snd sig) rT maxs maxl b et (phi C sig)) G"
 
 
 lemma wt_jvm_progD:
-  "wt_jvm_prog G phi ==> (\<exists>wt. wf_prog wt G)"
+  "wt_jvm_prog G phi \<Longrightarrow> (\<exists>wt. wf_prog wt G)"
   by (unfold wt_jvm_prog_def, blast)
 
 lemma wt_jvm_prog_impl_wt_instr:
-  "[| wt_jvm_prog G phi; is_class G C;
-      method (G,C) sig = Some (C,rT,maxs,maxl,ins,et); pc < length ins |] 
-  ==> wt_instr (ins!pc) G rT (phi C sig) maxs (length ins) et pc";
+  "\<lbrakk> wt_jvm_prog G phi; is_class G C;
+      method (G,C) sig = Some (C,rT,maxs,maxl,ins,et); pc < length ins \<rbrakk> 
+  \<Longrightarrow> wt_instr (ins!pc) G rT (phi C sig) maxs (length ins) et pc";
   by (unfold wt_jvm_prog_def, drule method_wf_mdecl, 
       simp, simp, simp add: wf_mdecl_def wt_method_def)
 
 lemma wt_jvm_prog_impl_wt_start:
-  "[| wt_jvm_prog G phi; is_class G C;
-      method (G,C) sig = Some (C,rT,maxs,maxl,ins,et) |] ==> 
+  "\<lbrakk> wt_jvm_prog G phi; is_class G C;
+      method (G,C) sig = Some (C,rT,maxs,maxl,ins,et) \<rbrakk> \<Longrightarrow> 
   0 < (length ins) \<and> wt_start G C (snd sig) maxl (phi C sig)"
   by (unfold wt_jvm_prog_def, drule method_wf_mdecl, 
       simp, simp, simp add: wf_mdecl_def wt_method_def)
