src/HOL/MicroJava/BV/Typing_Framework.thy
@@ -15,23 +15,23 @@ types
   's step_type = "nat \<Rightarrow> 's \<Rightarrow> (nat \<times> 's) list"
 
 constdefs
- bounded :: "'s step_type => nat => bool"
+ bounded :: "'s step_type \<Rightarrow> nat \<Rightarrow> bool"
 "bounded step n == !p<n. !s. !(q,t):set(step p s). q<n"  
 
- stable :: "'s ord => 's step_type => 's list => nat => bool"
+ stable :: "'s ord \<Rightarrow> 's step_type \<Rightarrow> 's list \<Rightarrow> nat \<Rightarrow> bool"
 "stable r step ss p == !(q,s'):set(step p (ss!p)). s' <=_r ss!q"
 
- stables :: "'s ord => 's step_type => 's list => bool"
+ stables :: "'s ord \<Rightarrow> 's step_type \<Rightarrow> 's list \<Rightarrow> bool"
 "stables r step ss == !p<size ss. stable r step ss p"
 
- is_bcv :: "'s ord => 's => 's step_type 
-           => nat => 's set => ('s list => 's list) => bool"  
+ is_bcv :: "'s ord \<Rightarrow> 's \<Rightarrow> 's step_type 
+           \<Rightarrow> nat \<Rightarrow> 's set \<Rightarrow> ('s list \<Rightarrow> 's list) \<Rightarrow> bool"  
 "is_bcv r T step n A bcv == !ss : list n A.
    (!p<n. (bcv ss)!p ~= T) =
    (? ts: list n A. ss <=[r] ts & wt_step r T step ts)"
 
  wt_step ::
-"'s ord => 's => 's step_type => 's list => bool"
+"'s ord \<Rightarrow> 's \<Rightarrow> 's step_type \<Rightarrow> 's list \<Rightarrow> bool"
 "wt_step r T step ts ==
  !p<size(ts). ts!p ~= T & stable r step ts p"
 
